tuplekey/stringlist.h
@@ -1,7 +1,0 @@
-
-typedef struct stringlist *stringlist_t;
-
-stringlist_t stringlist_new(void);
-
-void *stringlist_insert(stringlist_t p, char *key, void *value);
-void *stringlist_lookup(stringlist_t p, char *key);
