verif/indices/stringlist_instance.v
@@ -1,17 +1,50 @@
 Require Import VST.floyd.functional_base VST.floyd.proofauto.
 Require Import VST.floyd.library.
 Require Import stringlist.
-Require Import interface.
+Require Import unordered_interface.
 Require Import unordered_flat.
 Require Import verif_stringlist.
+Require Import definitions.
 
 Import UnorderedIndex.
 
+Lemma in_whole_in_fst: forall a l,
+  SetoidList.InA (stringlist.Raw.PX.eqk (elt:=V)) a l -> In (fst a) (map fst l).
+Proof. 
+  intros. induction l.
+  - inversion H; inversion H0; inversion H2.
+  - simpl. apply SetoidList.InA_cons in H. inversion H; clear H.
+     + left. destruct a, a0. inversion H0. simpl in H. subst. auto.
+     + right. auto.
+Qed. 
+
+Lemma notin_whole_notin_fst:  forall a l,
+   ~SetoidList.InA (stringlist.Raw.PX.eqk (elt:=V)) a l -> ~In (fst a) (map fst l).
+Proof.
+  intros. induction l.
+  - unfold not. intros. inversion H0.
+  - simpl.
+     rewrite SetoidList.InA_cons in H.
+     apply Classical_Prop.not_or_and in H.
+     apply Classical_Prop.and_not_or. split.
+     + inversion H; clear H. 
+        unfold stringlist.Raw.PX.eqk in H0. auto.
+     + inversion H; clear H. auto.
+Qed.
+
 Lemma lstnodup: forall lst, NoDup (map fst (stringlist.elements (elt:=V) lst)).
 Proof. 
-  intros. induction (stringlist.elements (elt:=V) lst).
+  intros. assert 
+  (K: SetoidList.NoDupA (stringlist.Raw.PX.eqk (elt:=V)) (stringlist.this lst)).
+  apply stringlist.NoDup.
+  assert (M: (stringlist.this lst) = (stringlist.elements (elt:=V) lst)) by auto.
+  rewrite M in K. clear M.
+  induction (stringlist.elements (elt:=V) lst); auto.
   - simpl. apply NoDup_nil.
-  - simpl. apply NoDup_cons; auto. Admitted.
+  - simpl. inversion K; subst. apply IHl in H2.
+     apply NoDup_cons; auto. clear H2 K IHl.
+     apply notin_whole_notin_fst. auto.
+Qed.
 
 Definition stringlist_index : index :=
   {| key := stringlist.key;
@@ -26,17 +59,18 @@ Definition stringlist_index : index :=
      t_repr := fun sh lst p => stringlist_rep lst p;
      t_type := t_stringlist;
      
+     create := stringlist.empty V;
+
      cursor_repr := fun mc p => emp;
 
      flatten := fun lst => mk_flat _  (stringlist.elements (elt:=V) lst) (lstnodup lst);
      
      insert := fun t k v => stringlist.add k v t;
 
-     delete := fun mc k => mc;
-
-      (* change lookup to be stringlist.find *)
-
    |}.
+
+Definition create_funspec := create_spec(stringlist_index).
+Definition stringlist_create_spec := (_stringlist_new, create_funspec).
 
 Definition lookup_funspec := lookup_spec(stringlist_index).
 Definition stringlist_lookup_spec := (_stringlist_lookup, lookup_funspec).
@@ -44,7 +78,18 @@ Definition stringlist_lookup_spec := (_stringlist_lookup, lookup_funspec).
 Definition insert_funspec := insert_spec(stringlist_index).
 Definition stringlist_insert_spec := (_stringlist_insert, insert_funspec).
 
-Definition Gprog : funspecs := [ new_scell_spec; strcmp_spec; stringlist_lookup_spec; stringlist_insert_spec ].
+Definition malloc_funspec := malloc_spec'.
+Definition malloc_spec := (_malloc, malloc_funspec).
+
+Definition exit_funspec := exit_spec'.
+Definition exit_spec := (_exit, exit_funspec).
+
+Definition cardinality_funspec := cardinality_spec(stringlist_index).
+Definition stringlist_cardinality_spec := (_stringlist_cardinality, cardinality_funspec).
+
+
+Definition Gprog : funspecs := [ new_scell_spec; strcmp_spec; malloc_spec;
+    exit_spec; stringlist_create_spec; stringlist_lookup_spec; stringlist_insert_spec ].
 
 (* ==================== HELPERS ==================== *)
 
@@ -104,7 +149,7 @@ Proof.
 Qed.
 
 Lemma find_middle: forall s lst1 lst2 v, ~ In s (map fst lst1 ++ map fst lst2) -> 
-                          @find stringlist.key unordered_flat.V Str_as_DT.eq_dec (lst1 ++ (s, v) :: lst2) s = Some v.
+                          @find stringlist.key V Str_as_DT.eq_dec (lst1 ++ (s, v) :: lst2) s = Some v.
 Proof. 
   induction lst1, lst2; intros.
   - simpl. destruct (Str_as_DT.eq_dec s s); auto. unfold Str_as_DT.eq in n. contradiction.
@@ -119,17 +164,74 @@ Proof.
 Qed.
 
 Lemma find_add: forall k v m,
-  @find stringlist.key unordered_flat.V Str_as_DT.eq_dec (stringlist.Raw.add k v (stringlist.this m)) k = Some v.
-Proof. Admitted.
+  @find stringlist.key V Str_as_DT.eq_dec (stringlist.Raw.add k v (stringlist.this m)) k = Some v.
+Proof. 
+  intros. induction (stringlist.this m).
+  - simpl. destruct (Str_as_DT.eq_dec k k); auto. unfold not in n. 
+     unfold Str_as_DT.eq in n. contradiction.
+  - simpl. destruct a. destruct (Str_as_DT.eq_dec k s).
+     + simpl. destruct (Str_as_DT.eq_dec k k); auto.
+        unfold not in n. unfold Str_as_DT.eq in n. contradiction.
+     + simpl. destruct (Str_as_DT.eq_dec s k). exfalso; apply n; auto.
+        rewrite IHt0. auto.
+Qed.
 
-Lemma list_byte_neq: forall s str, string_to_list_byte s <> string_to_list_byte str -> s <> str.
-Proof. Admitted.
+
+Lemma list_byte_neq: forall s str, 
+  string_to_list_byte s <> string_to_list_byte str -> s <> str.
+Proof.
+  intros. generalize dependent str. induction s.
+  - unfold not. intros. apply H. apply list_byte_eq in H0. auto.
+  - unfold not. intros. apply H. apply list_byte_eq. auto.
+Qed.
 
 Lemma notin_cons: forall k lst k0 (v0: V),
   ~ stringlist.Raw.PX.In k lst ->
   k0 <> k ->
   ~ stringlist.Raw.PX.In k (lst ++ [(k0, v0)]).
-Proof. Admitted.
+Proof.
+  intros. destruct lst.
+  - simpl. unfold stringlist.Raw.PX.In. unfold not. intros.
+     inversion H1. inversion H2; subst.
+     + inversion H4. simpl in H3. symmetry in H3. contradiction.
+     + inversion H4.
+  - simpl. unfold stringlist.Raw.PX.In. unfold not. intros.
+     inversion H1; clear H1. inversion H2; subst.
+     + inversion H3. destruct p; simpl in *; subst. apply H.
+         unfold stringlist.Raw.PX.In. exists v. auto.
+     + clear H3.
+         apply H. unfold stringlist.Raw.PX.In. exists x.
+         unfold stringlist.Raw.PX.MapsTo in *.
+         apply 
+         (@SetoidList.InA_app _ (stringlist.Raw.PX.eqke (elt:=V)) (p::lst) ([(k0,v0)]) (k, x)) 
+         in H2. inversion H2; clear H2; auto.
+         unfold not in H0. inversion H1; subst; inversion H3; subst; simpl in *.
+         symmetry in H2. contradiction.
+Qed.
+
+(* ==================== CREATE ==================== *)
+
+Lemma body_stringlist_create: semax_body Vprog Gprog 
+    f_stringlist_new stringlist_create_spec.
+Proof. 
+  unfold stringlist_create_spec. unfold create_funspec.
+  unfold create_spec.
+  start_function. 
+  forward_call (t_stringlist, gv).
+  { split3; auto. cbn. computable. }
+  Intros p. 
+  forward_if
+    (PROP ( )
+     LOCAL (temp _p p; gvars gv)
+     SEP (mem_mgr gv; malloc_token Ews t_stringlist p * data_at_ Ews t_stringlist p)).
+  { destruct eq_dec; entailer. }
+  { forward_call tt. entailer. }
+  { forward. rewrite if_false by assumption. entailer. }
+  { Intros. forward. forward. Exists p. Exists (stringlist.empty V).
+    entailer!. simpl.
+    unfold stringlist_rep. unfold stringlist.empty. simpl.
+    Exists (Vint (Int.repr 0)). entailer!. } 
+Qed.
 
 (* ==================== INSERT ==================== *)
 
@@ -175,7 +277,7 @@ Proof.
          apply H4 in M. rewrite M.
          (* create new cell with (k,v) *) 
          forward_call (gv, kptr, k, v, nullval, (@nil (string * V))).
-         Intros vret. Intros cp. forward. forward. Exists (stringlist.add k v m). entailer!. 
+         Intros vret. forward. forward. Exists (stringlist.add k v m). entailer!. 
          split. 
            { unfold lookup. simpl.
              rewrite find_add. auto. }
@@ -189,19 +291,18 @@ Proof.
              rewrite sepcon_assoc. rewrite sepcon_comm.
              replace (scell_rep [(k, v)] vret * data_at Ews (tptr t_scell) vret addr)
              with (strlst_rep addr vret [(k,v)]). sep_apply modus_ponens_wand.
-             replace (@stringlist.elements V
-             (@stringlist.add (@sig val is_pointer_or_null) k v m)) with (lst1 ++ [(k, v)]).
+             replace (@stringlist.elements V (@stringlist.add V k v m)) with (lst1 ++ [(k, v)]).
              unfold strlst_rep; entailer!.
              assert (K: data_at Ews (tptr t_scell) cp' mptr |-- data_at Ews t_stringlist cp' mptr).
             { (* this is where we need the extra premise of field_compatible *)
               unfold_data_at (data_at _ t_stringlist _ mptr). rewrite field_at_data_at.
               unfold field_address. if_tac; simpl; auto.
               * entailer!. * contradiction. } 
-             sep_apply K. clear K. entailer!. { admit. (* handle malloc token *)}
+             sep_apply K. clear K. entailer!. 
             { autorewrite with sublist in H. simpl. unfold stringlist.elements in H.
-              unfold stringlist.Raw.elements in H. 
-              assert (W: (@stringlist.this (@sig val is_pointer_or_null) m) = (@stringlist.this V m))
-              by (simpl; auto). rewrite W. rewrite <- H. apply notin_lst_add_end; auto. }
+              unfold stringlist.Raw.elements in H. rewrite <- H.
+              apply (@notin_lst_add_end lst1 k v) in H0.
+              rewrite <- H0. reflexivity. }
             { unfold strlst_rep. apply sepcon_comm. }}
              
       (* if list nonempty *)
@@ -221,7 +322,7 @@ Proof.
                 simpl. entailer!.
                 { unfold lookup. simpl. rewrite <- H. simpl in k.
                   assert 
-                  (P: @find stringlist.key unordered_flat.V Str_as_DT.eq_dec (lst1 ++ (k, v0) :: lst2) k 
+                  (P: @find stringlist.key V Str_as_DT.eq_dec (lst1 ++ (k, v0) :: lst2) k 
                          = (Some v0)).
                         { assert (W: NoDup (map fst (stringlist.elements (elt:=V) m))).
                           apply lstnodup. rewrite <- H in W. rewrite map_app in W. simpl in W. 
@@ -236,10 +337,11 @@ Proof.
                 assert (M: cstring Ews (string_to_list_byte k) str_ptr *
                 malloc_token Ews t_scell cellptr2 *
                 data_at Ews t_scell (str_ptr, (V_repr v, q)) cellptr2 * 
+                malloc_token Ews (tarray tschar (Zlength (string_to_list_byte k) + 1)) str_ptr *
                 scell_rep lst2 q
                 |-- scell_rep ((k, v) :: lst2) cellptr2).
-                { unfold scell_rep at 2; fold scell_rep. Exists q str_ptr. unfold verif_stringlist.V_repr. 
-                  unfold V_repr. cancel. unfold cstring. unfold string_rep.
+                { unfold scell_rep at 2; fold scell_rep. Exists q str_ptr. 
+                  cancel. unfold cstring. unfold string_rep.
                   rewrite length_string_list_byte_eq. entailer!. }
                 sep_apply M. rewrite sepcon_comm.
                 rewrite sepcon_assoc. 
@@ -253,13 +355,12 @@ Proof.
                   unfold field_address. if_tac; simpl; auto.
                   * entailer!. * contradiction. }
                 sep_apply K; clear K; cancel. unfold key. 
-                replace (@stringlist.elements V (@stringlist.add unordered_flat.V k v m))
+                replace (@stringlist.elements V (@stringlist.add V k v m))
                 with (lst1 ++ (k, v) :: lst2).
                 entailer!. simpl.
                 unfold stringlist.elements in H.
                 unfold stringlist.Raw.elements in H. clear M. clear P. clear H3. 
-                assert (W: (@stringlist.this V m) = (@stringlist.this unordered_flat.V m))
-                by (simpl; auto). rewrite <- W. rewrite <- H.
+                rewrite <- H.
                 apply notin_lst_add_middle. auto. }}
               { forward. entailer!. 
                 Exists (lst1 ++ [(k0,v0)]) lst2 (offset_val 8 cellptr2) q. entailer!.
@@ -281,8 +382,10 @@ Proof.
                 assert (Q: (cstring Ews (string_to_list_byte k0) str_ptr *
                 (malloc_token Ews t_scell cellptr2 *
                 (field_at Ews t_scell [StructField _key] str_ptr cellptr2 *
-                (field_at Ews t_scell [StructField _value] (verif_stringlist.V_repr v0) cellptr2 *
-                data_at Ews (tptr t_scell) cellptr2 addr)))) *
+                (malloc_token Ews
+                (tarray tschar (Zlength (string_to_list_byte k0) + 1)) str_ptr * 
+                (field_at Ews t_scell [StructField _value] (V_repr v0) cellptr2 *
+                data_at Ews (tptr t_scell) cellptr2 addr))))) *
                 strlst_rep (offset_val 8 cellptr2) cpnew lst' |-- strlst_rep addr cellptr2 ((k0, v0) :: lst')).
                 { unfold strlst_rep. cancel. unfold scell_rep at 2; fold scell_rep.
                   Exists cpnew str_ptr. cancel.
@@ -291,9 +394,8 @@ Proof.
                   unfold_data_at (data_at _ _ _ cellptr2).
                   rewrite (field_at_data_at _ _ [StructField _next]), field_address_offset.
                   entailer!. auto. } sep_apply Q. sep_apply modus_ponens_wand. 
-                rewrite app_assoc_reverse. simpl. entailer!.
-
-Admitted.
+                rewrite app_assoc_reverse. simpl. entailer!. }}
+Qed.
 
 
 (* ==================== LOOKUP ==================== *)
@@ -315,92 +417,98 @@ Proof. unfold stringlist_lookup_spec. unfold lookup_funspec. unfold lookup_spec.
   LOCAL()
   SEP((mem_mgr gv * stringlist_rep lst p * string_rep str q))).
  (* invariant holds entering loop*) 
-  - unfold stringlist_rep. Intros cell_ptr. forward. Exists (@nil (string * V)) (stringlist.elements lst).
+  - unfold stringlist_rep. Intros cell_ptr. forward. 
+     Exists (@nil (string * V)) (stringlist.elements lst).
      Exists cell_ptr.
      unfold stringlist_hole_rep.
      Exists cell_ptr. autorewrite with sublist. entailer!.
-      + inversion H4. inversion H5.
-      + apply wand_refl_cancel_right.
+     { inversion H4. inversion H5. }
+     { apply wand_refl_cancel_right. }
   (* invariant holds in the loop *)
   - Intros lst1 lst2 p0. forward_if (p0 <> nullval).
-    + unfold stringlist_hole_rep. Intros cell_ptr. entailer!.
-    + forward. entailer!.
-    + (* break inv used *) unfold stringlist_hole_rep. Intros cell_ptr.
-        rewrite H1.  forward. entailer!.
-       * assert (K: nullval = nullval). auto. apply H5 in K. subst. autorewrite with sublist in H.
-         rewrite H in H0. replace (lookup stringlist_index m k) with interface.nullV; auto.
-         unfold lookup. simpl. simpl in k. simpl in m. apply notin_lst_find_none in H0.
-         assert 
-         (P: @find stringlist.key unordered_flat.V Str_as_DT.eq_dec (stringlist.elements (elt:=V) m) k = None).
-         { replace (@None unordered_flat.V) with (@None V); auto. rewrite <- H0.
-           apply stringlistfind_eq_find. }
-          rewrite P; auto.
-       * unfold stringlist_rep. Exists cell_ptr. cancel.
-         apply modus_ponens_wand.
-    + destruct lst2. 
+    { unfold stringlist_hole_rep. Intros cell_ptr. entailer!. }
+    { forward. entailer!. }
+    { (* break inv used *) unfold stringlist_hole_rep. Intros cell_ptr.
+      rewrite H1.  forward. entailer!.
+      { assert (K: nullval = nullval). auto. apply H5 in K. 
+        subst. autorewrite with sublist in H.
+        rewrite H in H0. replace (lookup stringlist_index m k) with nullV; auto.
+        unfold lookup. simpl. simpl in k. simpl in m. apply notin_lst_find_none in H0.
+        assert 
+        (P: @find stringlist.key V Str_as_DT.eq_dec (stringlist.elements (elt:=V) m) k = None).
+        { rewrite <- H0.
+          apply stringlistfind_eq_find. }
+          rewrite P; auto. }
+        { unfold stringlist_rep. Exists cell_ptr. cancel.
+         apply modus_ponens_wand. }}
+    { destruct lst2. 
         (* lst2 empty *)
-       * unfold stringlist_hole_rep. Intros cell_ptr.
-          unfold scell_rep; fold scell_rep. Intros. contradiction.
+       { unfold stringlist_hole_rep. Intros cell_ptr.
+         unfold scell_rep; fold scell_rep. Intros. contradiction. }
          (* lst2 not empty *)
-       * unfold stringlist_hole_rep. Intros cell_ptr. destruct p1.
-          unfold scell_rep at 1; fold scell_rep. Intros q0 str_ptr.
-          forward. 
-          forward_call (str_ptr, string_to_list_byte s, q, string_to_list_byte str).
-          { unfold cstring. unfold string_rep.
-            repeat rewrite length_string_list_byte_eq. cancel. }
-          Intros vret. forward_if.
+       { unfold stringlist_hole_rep. Intros cell_ptr. destruct p1.
+         unfold scell_rep at 1; fold scell_rep. Intros q0 str_ptr.
+         forward. 
+         forward_call (str_ptr, string_to_list_byte s, q, string_to_list_byte str).
+         { unfold cstring. unfold string_rep.
+           repeat rewrite length_string_list_byte_eq. cancel. }
+         Intros vret. forward_if.
+         { destruct (Int.eq_dec vret Int.zero) in H2.
+           { forward.
+              { unfold V in v. entailer!.
+                destruct v. auto. }
+              { forward. entailer!.
+                { assert (M: lookup stringlist_index m k = v).
+                  { apply list_byte_eq in H2; rewrite <- H2. unfold lookup. simpl in k. simpl in m.
+                    assert (K: stringlist.elements m = (elements (flatten stringlist_index m))) by auto.
+                    rewrite <- K. rewrite <- H. simpl.
+                    assert 
+                    (P: @find stringlist.key V Str_as_DT.eq_dec (lst1 ++ (s, v) :: lst2) s 
+                     = (Some v)).
+                    { assert (W: NoDup (map fst (stringlist.elements (elt:=V) m))).
+                      apply lstnodup. rewrite <- H in W. rewrite map_app in W. simpl in W. 
+                      apply (@NoDup_remove_2 string (map fst (lst1)) (map fst (lst2)) s) in W.
+                      apply find_middle; auto. }
+                    rewrite P. auto. } rewrite M; simpl; auto. } 
+                 simpl t_repr. simpl key_repr. unfold string_rep. unfold cstring at 2. rewrite length_string_list_byte_eq.
+                 cancel. unfold stringlist_rep. Exists cell_ptr. cancel.
+                 apply wand_sepcon_adjoint.
+                 assert (K: cstring Ews (string_to_list_byte s) str_ptr * malloc_token Ews t_scell p0 *
+                 data_at Ews t_scell (str_ptr, (V_repr v, q0)) p0 *
+                 malloc_token Ews (tarray tschar (Zlength (string_to_list_byte s) + 1)) str_ptr *
+                 scell_rep lst2 q0 |-- 
+                 scell_rep ((s, v) :: lst2) p0).
+                 { unfold scell_rep at 2; fold scell_rep. Exists q0 str_ptr.
+                   unfold cstring. unfold string_rep. rewrite length_string_list_byte_eq.
+                   cancel. }
+                  sep_apply K. apply wand_sepcon_adjoint. apply modus_ponens_wand. }}
+           { contradiction. }}
           { destruct (Int.eq_dec vret Int.zero) in H2.
-            -- forward.
-              ++ unfold V in v. entailer!.
-              destruct v. auto.
-              ++ forward. entailer!.
-                    { assert (M: lookup stringlist_index m k = v).
-                      { apply list_byte_eq in H2; rewrite <- H2. unfold lookup. simpl in k. simpl in m.
-                        assert (K: stringlist.elements m = (elements (flatten stringlist_index m))) by auto.
-                        rewrite <- K. rewrite <- H. simpl.
-                        assert 
-                        (P: @find stringlist.key unordered_flat.V Str_as_DT.eq_dec (lst1 ++ (s, v) :: lst2) s 
-                         = (Some v)).
-                        { assert (W: NoDup (map fst (stringlist.elements (elt:=V) m))).
-                          apply lstnodup. rewrite <- H in W. rewrite map_app in W. simpl in W. 
-                          apply (@NoDup_remove_2 string (map fst (lst1)) (map fst (lst2)) s) in W.
-                          apply find_middle; auto. }
-                        rewrite P. auto. } rewrite M; simpl; auto. } (* Set Printing All to see implicit args *)
-                     simpl t_repr. simpl key_repr. unfold string_rep. unfold cstring at 2. rewrite length_string_list_byte_eq.
-                     cancel. unfold stringlist_rep. Exists cell_ptr. cancel.
-                     apply wand_sepcon_adjoint.
-                     assert (K: cstring Ews (string_to_list_byte s) str_ptr * malloc_token Ews t_scell p0 *
-                     data_at Ews t_scell (str_ptr, (V_repr v, q0)) p0 * scell_rep lst2 q0 |-- 
-                     scell_rep ((s, v) :: lst2) p0).
-                     { unfold scell_rep at 2; fold scell_rep. Exists q0 str_ptr.
-                       unfold cstring. unfold string_rep. rewrite length_string_list_byte_eq.
-                       cancel. }
-                      sep_apply K. apply wand_sepcon_adjoint. apply modus_ponens_wand.
-            -- contradiction. }
-          { destruct (Int.eq_dec vret Int.zero) in H2.
-            -- contradiction.
-            -- abbreviate_semax. forward. Exists (lst1 ++ [(s, v)]) lst2.
-                 Exists q0. entailer!.
-                 ++ split.
-                    ** rewrite <- H. rewrite app_assoc_reverse. simpl. auto.
-                    ** unfold not. intros. unfold stringlist.Raw.PX.In in H13. 
-                        unfold stringlist.Raw.PX.In in H0. unfold not in H0.
-                        unfold stringlist.Raw.PX.MapsTo in H13. inversion H13. 
-                        rewrite SetoidList.InA_app_iff in H14. inversion H14.
-                        { unfold stringlist.Raw.PX.MapsTo in H0. apply H0. exists x. auto. }
-                        { inversion H15. inversion H17. simpl in H19. rewrite H19 in H2. 
-                          contradiction. inversion H17. }
-                  ++ unfold string_rep. unfold cstring at 2. rewrite length_string_list_byte_eq.
-                        cancel. unfold stringlist_hole_rep. Exists cell_ptr. 
-                        entailer!. apply wand_frame_intro'.
-                        apply wand_sepcon_adjoint. apply wand_frame_intro'.
-                        assert (K: cstring Ews (string_to_list_byte s) str_ptr * malloc_token Ews t_scell p0 *
-                        data_at Ews t_scell (str_ptr, (V_repr v, q0)) p0 * scell_rep lst2 q0 |-- 
-                        scell_rep ((s, v) :: lst2) p0).
-                        { unfold scell_rep at 2; fold scell_rep. Exists q0 str_ptr.
-                          unfold cstring. unfold string_rep. rewrite length_string_list_byte_eq.
-                          cancel. }
-                        sep_apply K. apply modus_ponens_wand. }
+            contradiction.
+            abbreviate_semax. forward. Exists (lst1 ++ [(s, v)]) lst2.
+            Exists q0. entailer!.
+            { split.
+              { rewrite <- H. rewrite app_assoc_reverse. simpl. auto. }
+              { unfold not. intros. unfold stringlist.Raw.PX.In in H14. 
+                unfold stringlist.Raw.PX.In in H0. unfold not in H0.
+                unfold stringlist.Raw.PX.MapsTo in H14. inversion H14. 
+                rewrite SetoidList.InA_app_iff in H15. inversion H15.
+                { unfold stringlist.Raw.PX.MapsTo in H0. apply H0. exists x. auto. }
+                { inversion H16. inversion H18. simpl in H20. rewrite H20 in H2. 
+                  contradiction. inversion H18. }}}
+             { unfold string_rep. unfold cstring at 2. rewrite length_string_list_byte_eq.
+               cancel. unfold stringlist_hole_rep. Exists cell_ptr. 
+               entailer!. apply wand_frame_intro'.
+               apply wand_sepcon_adjoint. apply wand_frame_intro'.
+               assert (K: cstring Ews (string_to_list_byte s) str_ptr * malloc_token Ews t_scell p0 *
+               data_at Ews t_scell (str_ptr, (V_repr v, q0)) p0 *
+               malloc_token Ews (tarray tschar (Zlength (string_to_list_byte s) + 1)) str_ptr * 
+               scell_rep lst2 q0 |-- 
+               scell_rep ((s, v) :: lst2) p0).
+               { unfold scell_rep at 2; fold scell_rep. Exists q0 str_ptr.
+                 unfold cstring. unfold string_rep. rewrite length_string_list_byte_eq.
+                 cancel. }
+               sep_apply K. apply modus_ponens_wand. }}}}
   (* invariant holds after loop *) (* break inv used *)
   - forward. entailer!. simpl. auto. 
 Qed.
