verif/tuplekey/verif_stringlist.v
@@ -11,19 +11,13 @@ Require Import VST.msl.wand_frame.
 Require Import VST.msl.iter_sepcon.
 Require Import VST.floyd.reassoc_seq.
 Require Import VST.floyd.field_at_wand.
+Require Import definitions.
 Instance CompSpecs : compspecs. make_compspecs prog. Defined.
 Definition Vprog : varspecs. mk_varspecs prog. Defined.
 
-Set Default Timeout 20. 
-Require Import VST.msl.iter_sepcon.
-Require Import VST.floyd.library.
+Set Default Timeout 20.
 
-Definition V := sig is_pointer_or_null. 
-Definition nullV: V := exist _ nullval mapsto_memory_block.is_pointer_or_null_nullval.
-Definition V_repr: V -> val := @proj1_sig _ _.
-Definition maybe {A: Type} (o: option A) (default: A) :=
-  match o with Some a => a | None => default end.
-
+(* ------------------------ DEFINITIONS ------------------------ *)
 
 (* string as a decidable type *)
 Module Str_as_DT <: DecidableType.
@@ -57,7 +51,6 @@ Fixpoint length (s : string) : nat :=
 Definition string_rep (s: string) (p: val) : mpred := !! (~ List.In Byte.zero (string_to_list_byte s)) &&
   data_at Ews (tarray tschar (Z.of_nat(length(s)) + 1)) (map Vbyte (string_to_list_byte s ++ [Byte.zero])) p.
 
-
 Lemma length_string_list_byte_eq:
   forall str: string, Z.of_nat (length str) = Zlength (string_to_list_byte str).
 Proof.
@@ -66,7 +59,6 @@ Proof.
   - unfold length; fold length. unfold string_to_list_byte; fold string_to_list_byte.
      autorewrite with sublist. rewrite <- IHstr. apply Nat2Z.inj_succ.
 Qed.
-
 
 Definition string_rep_local_facts:
   forall s p, string_rep s p |-- !! (is_pointer_or_null p /\ 
@@ -84,9 +76,11 @@ Hint Resolve string_rep_local_facts: saturate_local.
 Fixpoint scell_rep (l: list (string*V)) (p: val): mpred :=
   match l with
   | [] => !!(p = nullval) && emp
-  | (k, v) :: tl => EX q:val, EX str_ptr: val, malloc_token Ews t_scell p *
+  | (k, v) :: tl => EX q:val, EX str_ptr: val, 
+                    malloc_token Ews t_scell p *
                     data_at Ews t_scell (str_ptr, (V_repr v, q)) p *
                     string_rep k str_ptr *
+                    malloc_token Ews (tarray tschar (Z.of_nat (length k) + 1)) str_ptr *
                     scell_rep tl q
   end.
 
@@ -113,7 +107,12 @@ Definition stringlist_rep (lst: stringlist.t V) (p: val): mpred :=
   data_at Ews t_stringlist cell_ptr p *
   scell_rep elts cell_ptr.
 
-(* add stringlist rep local facts *)
+Definition stringlist_rep_local_facts:
+  forall lst p, stringlist_rep lst p |-- !! (is_pointer_or_null p).
+Proof.
+  intros. unfold stringlist_rep. Intros cell_ptr. entailer!.
+Qed.
+
 (* ------------------------ STRLIB SPECS ------------------------ *)
 
 Definition strcmp_spec :=
@@ -153,8 +152,6 @@ Definition strlen_spec :=
     LOCAL (temp ret_temp (Vptrofs (Ptrofs.repr (Zlength s))))
     SEP (cstring Ews s str).
 
-(* ------------------------------------------------------------- *)
-
 
 (* ------------------------ STRINGLIST.V SPECS ------------------------ *)
 
@@ -175,7 +172,7 @@ Definition copy_string_spec: ident * funspec :=
  DECLARE _copy_string
   WITH wsh: share, s : val, str : string, gv: globals
   PRE [ _s OF tptr tschar ]
-    PROP (0 <= (Z.of_nat (length str) + 1) <= Ptrofs.max_unsigned)
+    PROP ()
     LOCAL (temp _s s; gvars gv)
     SEP (string_rep str s; mem_mgr gv)
   POST [ tptr tschar ]
@@ -190,50 +187,68 @@ Definition new_scell_spec: ident * funspec :=
    DECLARE _new_scell
  WITH gv: globals, k: val, str: string, value: V, pnext: val, tl: list (string*V)
  PRE [ _key OF tptr tschar, _value OF tptr tvoid, _next OF tptr t_scell ] 
-   PROP( 0 <= Z.of_nat (length str) + 1 <= Ptrofs.max_unsigned )
+   PROP()
    LOCAL(gvars gv; temp _key k; temp _value (V_repr value); temp _next pnext)
    SEP(string_rep str k; scell_rep tl pnext; mem_mgr gv)
  POST [ tptr t_scell ] 
    EX p:val,
       PROP() 
       LOCAL(temp ret_temp p) 
-      SEP(EX cp: val,
-            string_rep str k * malloc_token Ews (tarray tschar (Z.of_nat (length str) + 1)) cp;
-            scell_rep ((str, value) :: tl) p; mem_mgr gv).
-
-
-
-Definition stringlist_lookup_spec: ident * funspec :=
-   DECLARE _stringlist_lookup
- WITH gv: globals, lst: stringlist.t V, key: Z, p: val, k: val, str: string
- PRE [ _p OF tptr t_stringlist, _key OF tptr tschar ] 
-   PROP()
-   LOCAL(gvars gv; temp _p p; temp _key k)
-   SEP(mem_mgr gv; stringlist_rep lst p * string_rep str k)
- POST [ tptr tvoid ] 
-      PROP() 
-      LOCAL(temp ret_temp (V_repr (maybe (stringlist.find str lst) nullV))) 
-      SEP(mem_mgr gv; stringlist_rep lst p * string_rep str k).
-
-Definition stringlist_insert_spec: ident * funspec :=
-   DECLARE _stringlist_insert
- WITH gv: globals, lst: stringlist.t V, p: val, k: val, str: string, valptr: val
- PRE [ _p OF tptr t_stringlist, _key OF tptr tschar, _value OF tptr tvoid ] 
-   PROP()
-   LOCAL(gvars gv; temp _p p; temp _key k; temp _value valptr)
-   SEP(mem_mgr gv; stringlist_rep lst p * string_rep str k)
- POST [ tptr tvoid ] 
-      PROP() 
-      LOCAL(temp ret_temp (V_repr (maybe (stringlist.find str lst) nullV))) 
-      SEP(mem_mgr gv; stringlist_rep lst p * string_rep str k).
+      SEP(string_rep str k * scell_rep ((str, value) :: tl) p; mem_mgr gv).
 
 Definition Gprog : funspecs :=
-        ltac:(with_library prog [ strcmp_spec; strcpy_spec; strlen_spec; 
-        stringlist_new_spec; copy_string_spec; new_scell_spec; stringlist_lookup_spec;
-        stringlist_insert_spec]).
+        ltac:(with_library prog [ strcmp_spec; strcpy_spec; strlen_spec;
+        stringlist_new_spec; copy_string_spec; new_scell_spec]).
 
 
-(* ------------------------------------------------------------- *)
+(* --------------------------HELPERS-------------------------- *)
+
+
+Lemma scell_rep_modus: forall lst1 lst2 q, scell_rep lst1 q * (scell_rep lst1 q -* scell_rep lst2 q) 
+      |-- scell_rep lst2 q.
+Proof. 
+  intros. apply wand_frame_elim'. entailer!.
+Qed.
+
+Definition stringlist_hole_rep (lst1: list (string * V)) (lst: stringlist.t V) (p: val) (q: val): mpred :=
+  EX cell_ptr: val,
+  malloc_token Ews t_stringlist p *
+  data_at Ews t_stringlist cell_ptr p *
+  (scell_rep lst1 q * (scell_rep lst1 q -* scell_rep (elements lst) cell_ptr)). 
+
+Lemma ascii_range: forall a, 0 <= Z.of_N (Ascii.N_of_ascii a) <= Byte.max_unsigned.
+Proof. 
+  intros. destruct a. destruct b, b0, b1, b2, b3, b4, b5, b6; simpl; rep_omega.
+Qed.
+
+Lemma list_byte_eq: forall s str, string_to_list_byte s = string_to_list_byte str <-> s = str.
+Proof. 
+  split.
+  { intros. generalize dependent str. induction s.
+  - intros. inversion H. destruct str.
+     + auto.
+     + inversion H1.
+  - intros. destruct str.
+     + inversion H.
+     + simpl in H. set (b:= Byte.repr (Z.of_N (Ascii.N_of_ascii a))) in *. 
+        set (b0:= Byte.repr (Z.of_N (Ascii.N_of_ascii a0))) in *. assert (K: b = b0) by congruence.
+        unfold b, b0 in K.
+        apply f_equal with (f:= Byte.unsigned) in K. rewrite !Byte.unsigned_repr in K.
+        apply N2Z.inj in K.
+        apply f_equal with (f:= Ascii.ascii_of_N) in K.
+        rewrite !Ascii.ascii_N_embedding in K. f_equal. auto. inversion H. auto.
+        apply ascii_range. apply ascii_range. }
+  { intros. f_equal. auto. }
+Qed.
+
+Lemma notin_lst_find_none:  forall str lst, 
+  ~ Raw.PX.In str (elements (elt:=V) lst) -> find (elt:=V) str lst = None.
+Proof.
+  intros. case_eq (find (elt := V) str lst).
+  - intros v hfind%find_2. unfold Raw.PX.In in H. unfold MapsTo in hfind. 
+     unfold not in H. exfalso. apply H. exists v. auto.
+  - intros. auto.
+Qed.
 
 
 (* ------------------------ BODY PROOFS ------------------------ *)
@@ -241,7 +256,10 @@ Definition Gprog : funspecs :=
 
 Lemma body_stringlist_new: semax_body Vprog Gprog f_stringlist_new stringlist_new_spec.
 Proof.
-  start_function.
+  start_function. 
+  (* Problem: malloc expects tulong
+      Am I just not importing Clightdefs.tulong? *)
+
   forward_call (t_stringlist, gv).
   { split3; auto. cbn. computable. }
   Intros p. 
@@ -266,9 +284,15 @@ Proof.
     assert (L: Z.of_nat (length str) = Zlength (string_to_list_byte str)).
     { apply length_string_list_byte_eq. }
     rewrite L. entailer!. 
-  - forward. forward_call (tarray tschar (Z.of_nat(length(str)) + 1), gv).
+  - forward. sep_apply cstring_local_facts. Intros.
+     forward_call (tarray tschar (Z.of_nat(length(str)) + 1), gv).
     + unfold cstring. simpl. entailer!. rewrite length_string_list_byte_eq. auto.
-    + split; auto. rewrite sizeof_tarray_tschar; auto. omega.
+    + split; auto. assert (M: 0 <= Zlength (string_to_list_byte str)). 
+        apply Zlength_nonneg. rewrite sizeof_tarray_tschar; auto; 
+        rewrite length_string_list_byte_eq. 
+        split. omega.
+        rewrite <- initialize.max_unsigned_modulus in H. omega.
+        omega.
     + autorewrite with norm. Intros p. forward_if (p <> nullval).
         if_tac; entailer!.
        * rewrite if_true by auto. forward_call tt. entailer!.
@@ -287,7 +311,7 @@ Qed.
 
 Lemma body_new_scell: semax_body Vprog Gprog f_new_scell new_scell_spec.
 Proof.
-  start_function.
+  start_function. 
   forward_call (t_scell, gv).
   { now compute. }
   Intros p. forward_if (p <> nullval).
@@ -297,165 +321,9 @@ Proof.
   - Intros. rewrite if_false by auto. Intros.
      forward_call (Ews, k, str, gv).
      Intros cp. forward. forward. forward. forward.
-     Exists p. entailer!. Exists cp. unfold scell_rep at 2; fold scell_rep.
-     cancel. Exists pnext cp. entailer!.
+     Exists p. entailer!. unfold scell_rep at 2; fold scell_rep.
+     Exists pnext cp. entailer!.
 Qed.
-
-Lemma scell_rep_modus: forall lst1 lst2 q, scell_rep lst1 q * (scell_rep lst1 q -* scell_rep lst2 q) 
-      |-- scell_rep lst2 q.
-Proof. 
-  intros. apply wand_frame_elim'. entailer!.
-Qed.
-
-Definition stringlist_hole_rep (lst1: list (string * V)) (lst: stringlist.t V) (p: val) (q: val): mpred :=
-  EX cell_ptr: val,
-  malloc_token Ews t_stringlist p *
-  data_at Ews t_stringlist cell_ptr p *
-  (scell_rep lst1 q * (scell_rep lst1 q -* scell_rep (elements lst) cell_ptr)). 
-
-Lemma ascii_range: forall a, 0 <= Z.of_N (Ascii.N_of_ascii a) <= Byte.max_unsigned.
-Proof. 
-  intros. destruct a. destruct b, b0, b1, b2, b3, b4, b5, b6; simpl; rep_omega.
-Qed.
-
-Lemma list_byte_eq: forall s str, string_to_list_byte s = string_to_list_byte str -> s = str.
-Proof. 
-  intros. generalize dependent str. induction s.
-  - intros. inversion H. destruct str.
-     + auto.
-     + inversion H1.
-  - intros. destruct str.
-     + inversion H.
-     + simpl in H. set (b:= Byte.repr (Z.of_N (Ascii.N_of_ascii a))) in *. 
-        set (b0:= Byte.repr (Z.of_N (Ascii.N_of_ascii a0))) in *. assert (K: b = b0) by congruence.
-        unfold b, b0 in K. Check Byte.unsigned_repr. Check f_equal.
-        apply f_equal with (f:= Byte.unsigned) in K. rewrite !Byte.unsigned_repr in K.
-        apply N2Z.inj in K.
-        apply f_equal with (f:= Ascii.ascii_of_N) in K.
-        rewrite !Ascii.ascii_N_embedding in K. f_equal. auto. inversion H. auto.
-        
-Admitted.
-
-Lemma notin_lst_find_none:  forall str lst, 
-  ~ Raw.PX.In str (elements (elt:=V) lst) -> find (elt:=V) str lst = None.
-Proof.
-  intros. case_eq (find (elt := V) str lst).
-  - intros v hfind%find_2. unfold Raw.PX.In in H. unfold MapsTo in hfind. 
-     unfold not in H. exfalso. apply H. exists v. auto.
-  - intros. auto.
-Qed.
-
-Lemma body_stringlist_lookup: semax_body Vprog Gprog f_stringlist_lookup stringlist_lookup_spec.
-Proof. 
-  start_function.
-  Intros. 
-  (* loop invariant *)
-  forward_loop 
-  (EX lst1: list (string * V), EX lst2: list (string * V), EX q: val,
-  PROP( lst1 ++ lst2 = elements lst /\ not (stringlist.Raw.PX.In str lst1)) 
-  LOCAL(temp _q q; temp _key k)
-  SEP(mem_mgr gv; stringlist_hole_rep lst2 lst p q * string_rep str k))
-  (* break cond *)
-  break: 
-  (PROP ((Vint (Int.repr 0) = V_repr (maybe (find (elt:=V) str lst) nullV))) 
-  LOCAL()
-  SEP((mem_mgr gv * stringlist_rep lst p * string_rep str k))).
- (* invariant holds entering loop*) 
-  - unfold stringlist_rep. Intros cell_ptr. forward. Exists (@nil (string * V)) (elements lst).
-     Exists cell_ptr.
-     unfold stringlist_hole_rep.
-     Exists cell_ptr. autorewrite with sublist. entailer!.
-      + inversion H4. inversion H5.
-      + apply wand_refl_cancel_right.
-  (* invariant holds in the loop *)
-  - Intros lst1 lst2 q. forward_if (q <> nullval).
-    + unfold stringlist_hole_rep. Intros cell_ptr. entailer!.
-    + forward. entailer!.
-    + (* break inv used *) unfold stringlist_hole_rep. Intros cell_ptr.
-        rewrite H1.  forward. entailer!.
-       * assert (K: nullval = nullval). auto. apply H5 in K. subst. autorewrite with sublist in H.
-         rewrite H in H0. replace (find (elt:=V) str lst) with (@None V).
-         simpl. auto.  symmetry. apply notin_lst_find_none in H0. auto.
-       * unfold stringlist_rep. Exists cell_ptr. cancel.
-         apply modus_ponens_wand.
-    + destruct lst2. 
-        (* lst2 empty *)
-       * unfold stringlist_hole_rep. Intros cell_ptr.
-          unfold scell_rep; fold scell_rep. Intros. contradiction.
-         (* lst2 not empty *)
-       * unfold stringlist_hole_rep. Intros cell_ptr. destruct p0.
-          unfold scell_rep at 1; fold scell_rep. Intros q0 str_ptr.
-          forward.
-          forward_call (str_ptr, string_to_list_byte s, k, string_to_list_byte str).
-          { unfold cstring. unfold string_rep.
-            repeat rewrite length_string_list_byte_eq. cancel. }
-          Intros vret. forward_if.
-          { destruct (Int.eq_dec vret Int.zero) in H2.
-            -- forward.
-              ++ unfold V in v. entailer!. destruct v. auto.
-              ++ unfold elements in H. unfold Raw.elements in H. forward. entailer!.
-                    { assert (K: find (elt:=V) str lst = Some v).
-                      { apply stringlist.find_1. unfold MapsTo. rewrite <- H.
-                        apply list_byte_eq in H2. rewrite H2.
-                        unfold Raw.PX.MapsTo. 
-                        apply SetoidList.InA_app_iff. right. auto. }
-                     rewrite K. simpl. auto. }
-                     unfold string_rep. unfold cstring at 2. rewrite length_string_list_byte_eq.
-                     cancel. unfold stringlist_rep. Exists cell_ptr. cancel.
-                     apply wand_sepcon_adjoint.
-                     assert (K: cstring Ews (string_to_list_byte s) str_ptr * malloc_token Ews t_scell q *
-                     data_at Ews t_scell (str_ptr, (V_repr v, q0)) q * scell_rep lst2 q0 |-- 
-                     scell_rep ((s, v) :: lst2) q).
-                     { unfold scell_rep at 2; fold scell_rep. Exists q0 str_ptr.
-                       unfold cstring. unfold string_rep. rewrite length_string_list_byte_eq.
-                       cancel. }
-                      sep_apply K. apply wand_sepcon_adjoint. apply modus_ponens_wand.
-            -- contradiction. }
-          { destruct (Int.eq_dec vret Int.zero) in H2.
-            -- contradiction.
-            -- abbreviate_semax. forward. Exists (lst1 ++ [(s, v)]) lst2.
-                 Exists q0. entailer!.
-                 ++ split.
-                    ** rewrite <- H. rewrite app_assoc_reverse. simpl. auto.
-                    ** unfold not. intros. unfold Raw.PX.In in H13. 
-                        unfold Raw.PX.In in H0. unfold not in H0.
-                        unfold Raw.PX.MapsTo in H13. inversion H13. 
-                        rewrite SetoidList.InA_app_iff in H14. inversion H14.
-                        { unfold Raw.PX.MapsTo in H0. apply H0. exists x. auto. }
-                        { inversion H15. inversion H17. simpl in H19. rewrite H19 in H2. 
-                          contradiction. inversion H17. }
-                  ++ unfold string_rep. unfold cstring at 2. rewrite length_string_list_byte_eq.
-                        cancel. unfold stringlist_hole_rep. Exists cell_ptr. 
-                        entailer!. apply wand_frame_intro'.
-                        apply wand_sepcon_adjoint. apply wand_frame_intro'.
-                        assert (K: cstring Ews (string_to_list_byte s) str_ptr * malloc_token Ews t_scell q *
-                        data_at Ews t_scell (str_ptr, (V_repr v, q0)) q * scell_rep lst2 q0 |-- 
-                        scell_rep ((s, v) :: lst2) q).
-                        { unfold scell_rep at 2; fold scell_rep. Exists q0 str_ptr.
-                          unfold cstring. unfold string_rep. rewrite length_string_list_byte_eq.
-                          cancel. }
-                        sep_apply K. apply modus_ponens_wand. }
-  (* invariant holds after loop *) (* break inv used *)
-  - forward. entailer!.
-Qed.
-
-
-Lemma body_stringlist_insert: semax_body Vprog Gprog f_stringlist_insert stringlist_insert_spec.
-Proof.
-  start_function. Intros. unfold stringlist_rep. Intros cell_ptr.
-  forward. forward_loop (PROP() LOCAL() SEP()).
-  - (* inv holds at enter *) admit.
-  - admit.
-Admitted.
-
-
-
-
-
-
-
-
-
 
 
 
