verif/indices/definitions.v
@@ -1,0 +1,8 @@
+Require Import VST.floyd.proofauto.
+Require Import VST.floyd.library.
+
+Definition V := sig is_pointer_or_null. 
+Definition nullV: V := exist _ nullval mapsto_memory_block.is_pointer_or_null_nullval.
+Definition V_repr: V -> val := @proj1_sig _ _.
+Definition maybe {A: Type} (o: option A) (default: A) :=
+  match o with Some a => a | None => default end.
